ring/CellI.v
@@ -3,16 +3,14 @@ Require Import CRIS.
 Require Import ImpPrelude.
 Require Import CellHeader.
 
-Set Implicit Arguments.
-
 Module CellI. Section CellI.
-  Context `{Σ : GRA}.
+  Context `{!crisG Γ Σ α β τ _S _I, !concGS}.
 
   (* Index of this Cell *)
   Variable idx : nat.
 
   (* Scopes and a member variable `cv` *)
-  Definition scopes := [CellHdr.mn idx].
+  Definition scopes : list string := [CellHdr.mn idx].
   Definition v_cv := (CellHdr.mn idx) ↯ "cv".
 
   (* Implementations of get and set *)
@@ -26,17 +24,16 @@ Module CellI. Section CellI.
       cput v_cv x;;;
       Ret ().
 
-  Definition fnsems : fnsems_type :=
-    [(Some (CellHdr.get idx), (false, wmask_all, scopes, (None, cfunU get)));
-     (Some (CellHdr.set idx), (false, wmask_all, scopes, (None, cfunU set)))].
+  Definition fnsems : fnsemmap :=
+    {[Some (CellHdr.get idx) := Some (msk_real (msk_scp scopes msk_true), (None, cfunU get));
+      Some (CellHdr.set idx) := Some (msk_real (msk_scp scopes msk_true), (None, cfunU set))]}.
 
   Program Definition smod : SMod.t := {|
     SMod.scopes := scopes;
     SMod.fnsems := fnsems;
-    SMod.initial_st := [(v_cv,tt↑)];
+    SMod.initial_st := {[v_cv := Some tt↑]};
   |}.
-  Solve All Obligations with prove_scope.
-  Next Obligation. prove_nodup. Qed.
+  Solve All Obligations with mod_tac.
 
-  Definition t := Seal.sealing CRIS (SMod.to_mod sp_none smod).
+  Definition t := SMod.to_mod ∅ smod.
 End CellI. End CellI.
